src/MiscCompilerPassesProofsExtra.v
@@ -26,8 +26,8 @@ Module Compilers.
   Module Subst01.
     Import MiscCompilerPassesProofs.Compilers.Subst01.
 
-    Definition Interp_Subst01 {t} e Hwf
-      := @Interp_Subst01 _ ident _ (@ident.interp) (@ident.interp_Proper) t e Hwf.
+    Definition Interp_Subst01 is_ident_always_live {t} e Hwf
+      := @Interp_Subst01 _ ident is_ident_always_live _ (@ident.interp) (@ident.interp_Proper) t e Hwf.
   End Subst01.
 
   Hint Resolve Subst01.Wf_Subst01 : wf_extra.
@@ -37,8 +37,8 @@ Module Compilers.
   Module DeadCodeElimination.
     Import MiscCompilerPassesProofs.Compilers.DeadCodeElimination.
 
-    Definition Interp_EliminateDead {t} e Hwf
-      := @Interp_EliminateDead _ ident _ (@ident.interp) (@ident.interp_Proper) t e Hwf.
+    Definition Interp_EliminateDead is_ident_always_live {t} e Hwf
+      := @Interp_EliminateDead _ ident is_ident_always_live _ (@ident.interp) (@ident.interp_Proper) t e Hwf.
   End DeadCodeElimination.
 
   Hint Resolve DeadCodeElimination.Wf_EliminateDead : wf_extra.
